Contracts/Owned/Proofs/Basic.lean
@@ -66,10 +66,12 @@ theorem setStorageAddr_preserves_context (s : ContractState) (addr : Address) :
 theorem constructor_meets_spec (s : ContractState) (initialOwner : Address) :
   let s' := ((setStorageAddr owner initialOwner).run s).snd
   constructor_spec initialOwner s s' := by
-  simp [constructor_spec, owner, setStorageAddr, Specs.sameStorageMapContext,
-    Specs.sameStorage, Specs.sameStorageMap, Specs.sameContext]
-  intro slotIdx h_neq
-  simp [h_neq]
+  refine ⟨?_, ?_, ?_⟩
+  · simp [constructor_spec, owner, setStorageAddr]
+  · intro slotIdx h_neq
+    simp [constructor_spec, owner, setStorageAddr, h_neq]
+  · simp [constructor_spec, owner, setStorageAddr, Specs.sameStorageMapContext,
+      Specs.sameStorage, Specs.sameStorageMap, Specs.sameContext]
 
 theorem constructor_sets_owner (s : ContractState) (initialOwner : Address) :
   let s' := ((setStorageAddr owner initialOwner).run s).snd
@@ -140,10 +142,12 @@ theorem transferOwnership_meets_spec_when_owner (s : ContractState) (newOwner : 
   let s' := ((transferOwnership newOwner).run s).snd
   transferOwnership_spec newOwner s s' := by
   rw [transferOwnership_unfold s newOwner h_is_owner]
-  simp [transferOwnership_spec, ContractResult.snd, Specs.sameStorageMapContext,
-    Specs.sameStorage, Specs.sameStorageMap, Specs.sameContext]
-  intro slotIdx h_neq
-  simp [h_neq]
+  refine ⟨?_, ?_, ?_⟩
+  · simp [transferOwnership_spec, ContractResult.snd]
+  · intro slotIdx h_neq
+    simp [transferOwnership_spec, ContractResult.snd, h_neq]
+  · simp [transferOwnership_spec, ContractResult.snd, Specs.sameStorageMapContext,
+      Specs.sameStorage, Specs.sameStorageMap, Specs.sameContext]
 
 theorem transferOwnership_changes_owner_when_allowed (s : ContractState) (newOwner : Address)
   (h_is_owner : s.sender = s.storageAddr 0) :
